main-results/VCGEndToEnd.thy
@@ -293,6 +293,84 @@ lemma custom_context_tcfe_eq:
   apply (case_tac "f = field_val")
   by (simp_all add: sem_fields_def vints_def)
 
+lemma no_trace_atrue:
+  assumes "\<omega> \<in> atrue \<Delta> tys"
+  shows "get_trace |\<omega>| = (\<lambda>x. None)"
+  using assms unfolding atrue_def no_trace_def
+  by (simp add: core_charact_equi(3))
+
+
+lemma no_assert_assume_havoc_list:
+  "ConcreteSemantics.no_assert_assume (ConcreteSemantics.havoc_list l)"
+  by (induct l) simp_all
+
+lemma valid_then_no_assume_assert:
+  "ConcreteSemantics.no_assert_assume (fst (translate \<Delta> tys C))"
+  by (induct C) (simp_all add: Let_def no_assert_assume_havoc_list)
+
+lemma valid_then_no_assume_assert_snd:
+  assumes "Cv \<in> snd (translate \<Delta> tys C)"
+  shows "ConcreteSemantics.no_assert_assume Cv"
+  using assms
+  apply (induct C) apply (simp_all add: Let_def)
+  by (elim disjE; simp_all add: Let_def valid_then_no_assume_assert no_assert_assume_havoc_list)+
+
+lemma mono_custom_holds:
+  "ConcreteSemantics.mono_custom \<Gamma>"
+proof -
+  have "\<And>C \<omega> \<omega>' S. \<omega>' \<succeq> \<omega> \<Longrightarrow> red_custom_stmt \<Gamma> C \<omega> S \<Longrightarrow> wf_custom_stmt \<Gamma> C \<Longrightarrow> (\<exists>S'. red_custom_stmt \<Gamma> C \<omega>' S' \<and> S' \<ggreater> S)"
+  proof -
+    fix C \<omega> \<omega>' S
+    show "red_custom_stmt \<Gamma> C \<omega> S \<Longrightarrow> \<omega>' \<succeq> \<omega> \<Longrightarrow> wf_custom_stmt \<Gamma> C  \<Longrightarrow> (\<exists>S'. red_custom_stmt \<Gamma> C \<omega>' S' \<and> S' \<ggreater> S)"
+    proof (induct rule: red_custom_stmt.induct)
+      case (RedFieldAssign r \<omega> hl e v f \<Delta> ty)
+      moreover have "red_custom_stmt \<Delta> (custom.FieldAssign r f e) \<omega>' {update_heap_val \<omega>' (hl, f) v}"
+        apply (rule red_custom_stmt.RedFieldAssign)
+        using wf_expE[of r \<omega>' \<omega> hl]
+        using calculation(1) calculation(6) calculation(7) apply fastforce
+        apply (meson calculation(2) calculation(6) calculation(7) wf_custom_stmt.simps wf_expE)
+        using calculation(3) calculation(6) larger_mask_full apply blast
+        using RedFieldAssign by simp_all
+      moreover have "update_heap_val \<omega>' (hl, f) v \<succeq> update_heap_val \<omega> (hl, f) v"
+        apply (intro greater_prodI vstate_greater_charact1 greaterI)
+         apply (metis calculation(6) fstI greater_charact set_state_def succ_refl)
+          apply (simp add: calculation(6) greater_Ag greater_state_has_greater_parts(2) set_state_def)
+         apply (metis calculation(6) get_state_def get_state_set_state get_vh_vm_set_value(2) greaterE greater_state_has_greater_parts(3) vstate_greater_charact)
+        apply (case_tac "(hl, f) = l")
+        unfolding set_value_def
+         apply simp_all
+         apply (metis fun_upd_same get_state_def get_state_set_state get_vh_vm_set_value(1) set_value.abs_eq succ_refl)
+        by (metis (no_types, lifting) calculation(6) fun_upd_apply get_state_def get_state_set_state get_vh_Some_greater get_vh_vm_set_value(1) option_greater_iff set_value.abs_eq succ_refl)
+      then show "\<exists>S'. red_custom_stmt \<Delta> (custom.FieldAssign r f e) \<omega>' S' \<and> S' \<ggreater> {update_heap_val \<omega> (hl, f) v}"
+        by (meson calculation(8) greater_set_singleton)
+    qed
+  qed
+  then show ?thesis unfolding ConcreteSemantics.mono_custom_def by blast
+qed
+
+lemma stabilize_core_initial_state:
+  assumes "typed (tcfe \<Delta> tys) \<omega>"
+      and "get_trace |\<omega>| = (\<lambda>x. None)"
+    shows "stabilize |\<omega>| \<in> initial_vcg_states_equi (t2a_ctxt (default_ctxt (interp.domains \<Delta>) mdecl) (nth_option tys))"
+proof -
+  have fst_tcfes_eq: "fst (tcfes tys) = nth_option tys"
+    unfolding type_ctxt_front_end_syntactic_def by auto
+  show ?thesis
+    unfolding initial_vcg_states_equi_def apply simp
+    apply (rule conjI)
+     defer
+    apply (rule conjI)
+      defer
+    apply (simp add: core_charact_equi(2) core_structure(1) zero_mask_def)
+    unfolding t2a_ctxt_def TypedEqui.typed_def TypedEqui.typed_store_def
+     apply simp
+     apply (rule conjI)
+    apply (metis abs_type_context.simps(1) assms(1) default_ctxt_def fst_tcfes_eq make_context_semantic_def make_context_semantic_type_ctxt total_context.simps(3) type_ctxt_front_end_def typed_then_store_typed)
+    unfolding sem_fields_def absval_interp_total_def
+     apply simp
+     apply (metis TypedEqui.typed_core TypedEqui.typed_def TypedEqui.typed_state_axioms assms(1) custom_context_tcfe_eq sem_fields_def typed_state.typed_state_then_stabilize_typed)
+    using assms(2) by blast
+qed
 
 theorem sound_syntactic_translation_VCG:
   assumes "wf_stmt \<Delta> tys C"
@@ -320,11 +398,14 @@ theorem sound_syntactic_translation_VCG:
 
       and "P = make_semantic_assertion_gen False \<Delta> (tcfes tys) Ps"
       and "Q = make_semantic_assertion_gen False \<Delta> (tcfes tys) Qs"     
-    shows "tcfe \<Delta> tys \<turnstile>CSL [P \<otimes> UNIV] C [Q \<otimes> UNIV]"
-proof (rule sound_syntactic_translation[OF assms(1-2) _ _ assms(3)])
-  show "ConcreteSemantics.wf_abs_stmt (tcfe \<Delta> tys) (fst (translate \<Delta> tys C))"
-    by (simp add: assms(1) assms(2) wf_stmt_implies_wf_translation)
-  show "\<And>Cv. Cv \<in> snd (translate \<Delta> tys C) \<Longrightarrow> ConcreteSemantics.wf_abs_stmt (tcfe \<Delta> tys) Cv"
+    shows "tcfe \<Delta> tys \<turnstile>CSL [P \<otimes> atrue \<Delta> tys] C [Q \<otimes> atrue \<Delta> tys]"
+
+proof (rule sound_translation[OF assms(1-3)])
+
+  have wf_fst: "ConcreteSemantics.wf_abs_stmt (tcfe \<Delta> tys) (fst (translate \<Delta> tys C))"
+    using assms(1) assms(2) wf_stmt_implies_wf_translation by blast
+
+  have wf_snd: "\<And>Cv. Cv \<in> snd (translate \<Delta> tys C) \<Longrightarrow> ConcreteSemantics.wf_abs_stmt (tcfe \<Delta> tys) Cv"
     using assms(1) assms(2) wf_stmt_implies_wf_translation_snd by blast
 
   have tcfe_eq: "variables (tcfe \<Delta> tys) = nth_option (map (set_from_type (domains \<Delta>)) tys)"
@@ -338,8 +419,7 @@ proof (rule sound_syntactic_translation[OF assms(1-2) _ _ assms(3)])
   let ?\<Lambda> = "nth_option tys"
   let ?Ctr_mainV = "(stmt.Seq (stmt.Seq (stmt.Inhale Ps) ?Ctr_main) (stmt.Exhale Qs))"
 
-  show "ConcreteSemantics.verifies_set (tcfe \<Delta> tys) (atrue \<Delta> tys)
-    (abs_stmt.Inhale P ;; compile False \<Delta> (tcfes tys) ?Ctr_main ;; abs_stmt.Exhale Q)"
+  show "ConcreteSemantics.verifies_set (tcfe \<Delta> tys) (atrue \<Delta> tys) (abs_stmt.Inhale P ;; fst (translate \<Delta> tys C) ;; abs_stmt.Exhale Q)"
   proof -
 
     have A1: "ConcreteSemantics.verifies_set (t2a_ctxt ?ctxt ?\<Lambda>) (initial_vcg_states_equi (t2a_ctxt ?ctxt ?\<Lambda>))
@@ -385,21 +465,66 @@ proof (rule sound_syntactic_translation[OF assms(1-2) _ _ assms(3)])
         by metis
     qed
 
-    hence "ConcreteSemantics.verifies_set (tcfe \<Delta> tys) (initial_vcg_states_equi (t2a_ctxt ?ctxt ?\<Lambda>))
+    hence r: "ConcreteSemantics.verifies_set (tcfe \<Delta> tys) (initial_vcg_states_equi (t2a_ctxt ?ctxt ?\<Lambda>))
               (abs_stmt.Inhale P ;; compile False \<Delta> (tcfes tys) ?Ctr_main ;; abs_stmt.Exhale Q)"
       using \<open>P = _\<close> \<open>Q = _\<close>
       by simp
 
-    thus ?thesis
-      sorry \<comment>\<open>Thibault: TODO monotonicity etc...\<close>     
-  qed
 
+    show "ConcreteSemantics.verifies_set (tcfe \<Delta> tys) (atrue \<Delta> tys) (abs_stmt.Inhale P ;; fst (translate \<Delta> tys C) ;; abs_stmt.Exhale Q)"
+      apply (rule ConcreteSemantics.verifies_setI)
+      apply (rule ConcreteSemantics.monotonicity_verifiesE)
+           apply (simp_all; intro conjI)
+             apply (simp_all add: assms(3) assms(12) wf_fst)
+      using assms(12) assms(3) apply blast
+         defer
+         defer
+         defer
+         apply (subgoal_tac "\<omega> \<succeq> stabilize |\<omega>| ")
+          apply assumption
+         apply (metis already_stable core_stabilize_mono(2) max_projection_prop_pure_core mpp_smaller)
+        defer
+        defer
+      apply (rule verifies_more_verifies)
+         apply (rule verifies_more_seq)+
+             apply (rule verifies_more_refl)
+      apply (rule translation_refinement_syntactic_semantic(1)[OF assms(2) assms(1) wf_fst wf_snd])
+            apply (simp_all add: assms)
+      using assms(12) assms(3) apply blast
+        apply (rule verifies_more_refl)
+      using wf_fst assms(12) assms(3) apply argo
+    proof -
+      fix \<omega> assume asm0: "\<omega> \<in> atrue \<Delta> tys" "sep_algebra_class.stable \<omega>" "typed (tcfe \<Delta> tys) \<omega>"
+      moreover have "stabilize |\<omega>| \<in> initial_vcg_states_equi (t2a_ctxt ?ctxt ?\<Lambda>)"
+        apply (rule stabilize_core_initial_state)
+        apply (simp add: calculation(3))
+        using calculation(1) no_trace_atrue by blast
+    then show "ConcreteSemantics.verifies (tcfe \<Delta> tys)
+          (abs_stmt.Inhale (make_semantic_assertion_untyped \<Delta> (tcfes tys) Ps) ;; compile False \<Delta> (tcfes tys) (fst (translate_syn C)) ;;
+           abs_stmt.Exhale (make_semantic_assertion_untyped \<Delta> (tcfes tys) Qs))
+          (stabilize |\<omega>| )"
+        by (metis ConcreteSemantics.verifies_set_def TypedEqui.typed_core TypedEqui.typed_state_then_stabilize_typed assms(12) assms(13) calculation(3) r stabilize_is_stable)
+      
+      show "typed (tcfe \<Delta> tys) (stabilize |\<omega>| )"
+        using TypedEqui.typed_core TypedEqui.typed_state_then_stabilize_typed calculation(3) by blast
+      show "ConcreteSemantics.no_assert_assume (fst (translate \<Delta> tys C))"
+        using valid_then_no_assume_assert by blast
+      show "ConcreteSemantics.mono_custom (tcfe \<Delta> tys)"
+        by (simp add: mono_custom_holds)
+    qed
+  qed
 
   fix Cv
   
-  assume "Cv \<in> compile False \<Delta> (tcfes tys) ` snd (translate_syn C)"
-  from this obtain Cv_syn where "Cv_syn \<in> snd (translate_syn C)" and "Cv = compile False \<Delta> (tcfes tys) Cv_syn"
-    by blast
+  assume "Cv \<in> snd (translate \<Delta> tys C)"
+
+  have "verifies_more_set (tcfe \<Delta> tys) (snd (translate \<Delta> tys C)) (compile False \<Delta> (tcfes tys) ` snd (translate_syn C))"
+    apply (rule translation_refinement_syntactic_semantic(2)[OF assms(2) assms(1)])
+    using wf_fst wf_snd by force+
+  then obtain Cv_syn where ver_more: "Cv_syn \<in> snd (translate_syn C)" "verifies_more (tcfe \<Delta> tys) Cv (compile False \<Delta> (tcfes tys) Cv_syn)"
+    using \<open>Cv \<in> snd (translate \<Delta> tys C)\<close> assms(1) assms(2) translation_refinement_snd wf_fst wf_snd by blast
+
+
   let ?mdeclAux = "triple_as_method_decl tys 
                               true_syn_assertion Cv_syn true_syn_assertion"
   let ?ctxt = "(default_ctxt (domains \<Delta>) ?mdeclAux) :: int total_context"
@@ -409,9 +534,11 @@ proof (rule sound_syntactic_translation[OF assms(1-2) _ _ assms(3)])
     using AuxiliaryMethodsCorrectAndTyped[OF \<open>Cv_syn \<in> _\<close>, simplified Let_def]    
     by (auto intro!: stmt_typing.intros
                         assertion_typing.intros atomic_assertion_typing.intros pure_exp_typing.intros)
+
+
   show "ConcreteSemantics.verifies_set (tcfe \<Delta> tys) (atrue \<Delta> tys) Cv"
   proof -
-    have "ConcreteSemantics.verifies_set (t2a_ctxt ?ctxt ?\<Lambda>) (initial_vcg_states_equi (t2a_ctxt ?ctxt ?\<Lambda>))
+    have ver1: "ConcreteSemantics.verifies_set (t2a_ctxt ?ctxt ?\<Lambda>) (initial_vcg_states_equi (t2a_ctxt ?ctxt ?\<Lambda>))
                (compile False (ctxt_to_interp ?ctxt) (?\<Lambda>, declared_fields (program_total ?ctxt)) 
                (stmt.Seq (stmt.Seq (stmt.Inhale true_syn_assertion) Cv_syn) (stmt.Exhale true_syn_assertion)))"
       apply (rule VCG_to_verifies_set)
@@ -424,9 +551,17 @@ proof (rule sound_syntactic_translation[OF assms(1-2) _ _ assms(3)])
        apply force
        by (simp_all add: default_ctxt_def AbsTypeWf ValidPrePost)
 
-    hence A1: "ConcreteSemantics.verifies_set (t2a_ctxt ?ctxt ?\<Lambda>) (initial_vcg_states_equi (t2a_ctxt ?ctxt ?\<Lambda>))
+   moreover have A1: "ConcreteSemantics.verifies_set (t2a_ctxt ?ctxt ?\<Lambda>) (initial_vcg_states_equi (t2a_ctxt ?ctxt ?\<Lambda>))
                (compile False (ctxt_to_interp ?ctxt) (?\<Lambda>, declared_fields (program_total ?ctxt)) Cv_syn)"
-      sorry \<comment>\<open>TODO: Thibault --> remove inhale true exhale true\<close>
+     apply (rule ConcreteSemantics.inhale_c_exhale_verifies_simplifies[where
+         ?A="make_semantic_assertion_untyped (ctxt_to_interp ?ctxt) (?\<Lambda>, declared_fields (program_total ?ctxt)) true_syn_assertion" and
+         ?B="make_semantic_assertion_untyped (ctxt_to_interp ?ctxt) (?\<Lambda>, declared_fields (program_total ?ctxt)) true_syn_assertion"])
+      defer
+     using ver1 apply simp
+     unfolding make_semantic_assertion_gen_def apply simp
+     unfolding ctxt_to_interp_def red_pure_assert_def corely_def emp_core_def apply simp
+     by (metis core_is_pure pure_def red_pure_red_pure_exps.RedLit val_of_lit.simps(1))
+
 
     hence "ConcreteSemantics.verifies_set (tcfe \<Delta> tys) (initial_vcg_states_equi (t2a_ctxt ?ctxt ?\<Lambda>)) (compile False \<Delta> (tcfes tys) Cv_syn)"
     proof -
@@ -458,8 +593,29 @@ proof (rule sound_syntactic_translation[OF assms(1-2) _ _ assms(3)])
         by argo        
     qed
 
-    thus ?thesis
-      sorry \<comment>\<open>Thibault: TODO monotonicity etc...\<close>
+
+    show "ConcreteSemantics.verifies_set (tcfe \<Delta> tys) (atrue \<Delta> tys) Cv"
+      apply (rule ConcreteSemantics.verifies_setI)
+      apply (rule ConcreteSemantics.monotonicity_verifiesE)
+      using \<open>Cv \<in> snd (translate \<Delta> tys C)\<close> wf_snd apply blast
+      using mono_custom_holds apply blast
+      using valid_then_no_assume_assert_snd
+      using \<open>Cv \<in> snd (translate \<Delta> tys C)\<close> apply blast
+        apply (rule verifies_more_verifies[OF ver_more(2)])
+      defer
+          defer
+          defer
+      defer
+         apply (subgoal_tac "\<omega> \<succeq> stabilize |\<omega>|")
+           apply assumption
+          apply (metis already_stable core_stabilize_mono(2) max_projection_prop_pure_core mpp_smaller)
+         apply simp_all
+       apply (subgoal_tac "stabilize |\<omega>| \<in> initial_vcg_states_equi (t2a_ctxt ?ctxt ?\<Lambda>)")
+      apply (meson ConcreteSemantics.verifies_set_def TypedEqui.typed_core TypedEqui.typed_state_then_stabilize_typed \<open>ConcreteSemantics.verifies_set (tcfe \<Delta> tys) (initial_vcg_states_equi (t2a_ctxt (default_ctxt (interp.domains \<Delta>) (triple_as_method_decl tys true_syn_assertion Cv_syn true_syn_assertion)) (nth_option tys))) (compile False \<Delta> (tcfes tys) Cv_syn)\<close> stabilize_is_stable)
+      apply (rule stabilize_core_initial_state)
+        apply simp_all
+      using no_trace_atrue apply blast
+      using TypedEqui.typed_core TypedEqui.typed_state_then_stabilize_typed by blast
   qed
 qed
 
